Complete re-write of the Sieve of Eratosthenes
The existing implementation was missing a key constraint in the Sieve
structure. However, adding that constraint excludes the possibility of
a partially marked Sieve as exists during the execution of the
'mark_multiples' loop.

The solution was to create a separate state structure
(MarkMultiplesState) which is created from a Sieve. Then after
mark_multiples is complete, a new Sieve will be constructed from the
MarkMultiplesState.

Note that the current implementation is still incomplete and the
MarkMultiplesState may need one more constraint to allow for the
reconstruction of the Sieve.

FormalVerifyMisc/CodeChef/Template/Primes.lean
@@ -17,8 +17,8 @@ structure Sieve (L : ℕ) where
   divs : Array Int32
   -- The list of primes found thus far
   primes : Array Int32
-  -- The next prime to be added to the sieve
-  p : Int32
+  -- Current search location
+  i : Int32
   -- The size of 'divs' is given by 'L'
   hsize : divs.size = L
   -- The length of the sieve has an upper bound
@@ -26,36 +26,65 @@ structure Sieve (L : ℕ) where
   hLlt : L < 2^30
   -- The entries in the sieve are non-negative
   hdivsnn : ∀ x ∈ divs, 0 ≤ x
-  -- The values in 'primes' are all positive
-  hprimespos : ∀ q ∈ primes, 0 < q
-  -- 'p' is positive
-  hppos : 0 < p
-  -- 'p' is less than 'L' - the size of the sieve
-  hplt : p.toInt < (L : ℤ)
-  -- The absolute value of 'p' is prime
-  hpprime : Nat.Prime p.toInt.natAbs
-  -- Any prime less than 'p' is already in 'primes'
-  hpnext : ∀ q, Nat.Prime q → (q : ℤ) < p.toInt →
-    (q : ℤ) ∈ (Array.map Int32.toInt primes)
-  -- For every value 'q' in 'primes', every multiple of 'q' is marked in 'divs'
-  hmarked : ∀ q ∈ primes, ∀ i, (0 < i) → (ilt : i < divs.size) →
-    q.toInt ∣ (i : ℤ) → divs[i] ≠ 0
-  -- A natural number is in 'primes' if-and-only-if it is a prime
-  -- less than or equal to the last value in 'primes'
-  hpmem_iff : (hnnil : primes ≠ #[]) → ∀ q : ℕ,
-    ((q : ℤ) ∈ (Array.map Int32.toInt primes) ↔
-     (q : ℤ) ≤ (primes.back (Array.size_pos_iff.mpr hnnil)).toInt ∧ Nat.Prime q)
+  -- 'i' is positive
+  hipos : 0 < i.toInt
+  -- 'i' is less than or equal to 'L' - the size of the sieve
+  -- TODO: Do we actually need this?
+  hile : i.toInt ≤ (L : ℤ)
+  -- Each entry in the sieve is marked if-and-only-if its index
+  -- is divisible by some prime in 'primes'
+  hmarked : ∀ j, (0 < j) → (jlt : j < divs.size) →
+    (∃ p ∈ primes, p.toInt ∣ (j : ℤ)) ↔ divs[j] ≠ 0
+  -- A natural number is in 'primes' if-and-only-if
+  -- it is a prime less than 'i'
+  hpmem_iff : ∀ p : ℕ,
+    ((p : ℤ) ∈ (Array.map Int32.toInt primes) ↔
+     (p : ℤ) < i.toInt ∧ Nat.Prime p)
   -- If an entry in the sieve is non-zero, its value corresponds to the smallest
   -- divisor of its index greater than 1
-  hdivs_dvd : ∀ i, (ilt : i < divs.size) → divs[i]'(ilt) ≠ 0 →
-    (divs[i]'(ilt)).toInt ∣ i ∧
-    ∀ y, 1 < y → y ∣ i → (divs[i]'(ilt)).toInt ≤ (y : ℤ)
+  hdivs_dvd : ∀ j, (jlt : j < divs.size) → divs[j]'(jlt) ≠ 0 →
+    (divs[j]'(jlt)).toInt ∣ j ∧
+    ∀ y, 1 < y → y ∣ j → (divs[j]'(jlt)).toInt ≤ (y : ℤ)
+
+-- Show equivalence for the two ways of expressing the upper bound on an index into S.divs
+theorem lt_sieve_length_iff_of_nonneg
+  {L : ℕ} (S : Sieve L) (n : Int32) (hnnn : 0 ≤ n) :
+  n.toInt.natAbs < S.divs.size ↔ n.toInt < (L : ℤ) := by
+  rw [← Int.ofNat_lt]
+  rw [Int.ofNat_natAbs_of_nonneg (Int32.le_iff_toInt_le.mp hnnn), S.hsize]
+
+theorem lt_sieve_length_of_lt_index
+  {L : ℕ} {S : Sieve L} {j : ℕ} (jlt : (j : ℤ) < S.i.toInt) : j < S.divs.size := by
+  rw [S.hsize]
+  apply Int.lt_of_ofNat_lt_ofNat
+  apply lt_of_lt_of_le jlt S.hile
+
+-- Every entry properly between 1 and 'i' is marked
+-- This is the result of combining 'hmarked' (every entry with a divisor in
+-- 'primes' is marked) and 'hpmem_iff' (every prime less than S.i is in 'primes)
+theorem sieve_marked_of_lt_index {L : ℕ} (S : Sieve L) :
+  ∀ (j : ℕ), (ltj : 1 < j) → (jlt : (j : ℤ) < S.i.toInt) →
+  S.divs[j]'(lt_sieve_length_of_lt_index jlt) ≠ 0 := by
+  intro j ltj jlt
+  have jlt' := lt_sieve_length_of_lt_index jlt
+  -- Get some prime 'p' that divides 'j'
+  rcases Nat.exists_prime_and_dvd (ne_of_lt ltj).symm with ⟨p, pprime, pdvd⟩
+  have jpos : 0 < j := lt_trans (by simp) ltj
+  apply (S.hmarked j jpos jlt').mp
+  have ple := Nat.le_of_dvd jpos pdvd
+  have plt : (p : ℤ) < S.i.toInt :=
+    lt_of_le_of_lt (Int.ofNat_le_ofNat_of_le ple) jlt
+  -- Get the Int32 that corresponds to 'p' in 'primes' (it must exist by 'hpmem_iff')
+  rcases Array.exists_of_mem_map ((S.hpmem_iff p).mpr ⟨plt, pprime⟩) with ⟨p', p'mem, hp'p⟩
+  apply Int.ofNat_dvd.mpr at pdvd
+  use p', p'mem
+  rwa [hp'p]
 
 -- Construct a sieve with all elements set to zero
 def init_sieve : Sieve SIEVE_SIZE where
   divs := Array.replicate SIEVE_SIZE 0
   primes := #[]
-  p := 2
+  i := 2
   hsize := Array.size_replicate
   hLlt := by
     unfold SIEVE_SIZE;
@@ -63,602 +92,211 @@ def init_sieve : Sieve SIEVE_SIZE where
   hdivsnn := by
     intro x xmem
     rw [(Array.mem_replicate.mp xmem).2]; rfl
-  hprimespos :=
-    fun _ hmem ↦ False.elim (Array.not_mem_empty _ hmem)
-  hppos := rfl
-  hplt := by
+  hipos := by simp
+  hile := by
     unfold SIEVE_SIZE
     simp
-  hpprime := by
-    simp; norm_num
-  hpnext := by
-    intro q qprime qlt
-    absurd qlt; simp
-    exact Nat.Prime.two_le qprime
-  hmarked := by
-    intro _ pmem
-    exact False.elim (Array.not_mem_empty _ pmem)
-  hpmem_iff := fun h ↦ False.elim (h rfl)
+  hmarked := by simp
+  hpmem_iff := by
+    intro p; simp; intro plt
+    interval_cases p <;> norm_num
   hdivs_dvd := by
-    intro i ilt hnz
+    intro j jlt hnz
     constructor
     · absurd hnz; simp
     · intro y lty ydvd; simp
 
--- Update the sieve to indicate that 'p' is the smallest divisor of 'n'
-def mark_sieve {L : ℕ} (S : Sieve L) (n : Int32)
-  (hnpos : 0 < n)
-  (nlt : n.toInt.natAbs < S.divs.size)
-  (hdvd : S.p.toInt ∣ n.toInt) : Sieve L where
-  divs := if S.divs[n.toInt.natAbs] ≠ 0 then S.divs
-    else S.divs.set n.toInt.natAbs S.p nlt
-  primes := S.primes
-  p := S.p
-  hsize := by
-    split_ifs with h
-    · exact S.hsize
-    · rw [Array.size_set nlt]
-      exact S.hsize
-  hLlt := S.hLlt
-  hdivsnn := by
-    intro x
-    split_ifs with h
-    · intro xmem
-      exact S.hdivsnn x xmem
-    · intro xmem
-      rcases Array.mem_or_eq_of_mem_set xmem with lhs | rhs
-      · exact S.hdivsnn x lhs
-      · rw [rhs]
-        exact Int32.le_of_lt S.hppos
-  hprimespos := S.hprimespos
-  hppos := S.hppos
-  hplt := S.hplt
-  hpprime := S.hpprime
-  hpnext := S.hpnext
+-- Prove that a loop that terminates by showing that 'cur' increases by 'inc'
+-- on each iteration and that its absolute value never exceeds 'ub'.
+--
+-- TODO: This will likely be useful in other file as well
+-- consider moving it to a separate file.
+theorem termination_by_increasing_int32 (cur inc : Int32) (ub : ℕ)
+  (curpos : 0 < cur) (incpos : 0 < inc)
+  (curlt : cur.toInt < (ub : ℤ)) (inclt : inc.toInt < (ub : ℤ))
+  (uble : ub ≤ 2^30) :
+  ub - (cur + inc).toInt.natAbs < ub - cur.toInt.natAbs := by
+  have curpos' : 0 < cur.toInt := Int32.lt_iff_toInt_lt.mp curpos
+  have incpos' : 0 < inc.toInt := Int32.lt_iff_toInt_lt.mp incpos
+  rw [int32_toInt_add_of_add_bounds
+    (le_of_lt curpos')
+    (lt_of_lt_of_le curlt (Int.ofNat_le_ofNat_of_le uble))
+    (le_of_lt incpos')
+    (lt_of_lt_of_le inclt (Int.ofNat_le_ofNat_of_le uble))
+    (by simp) (by simp)]
+  rw [← Int.ofNat_natAbs_of_nonneg (le_of_lt curpos')] at curlt
+  apply Nat.sub_lt_sub_left (Int.lt_of_ofNat_lt_ofNat curlt)
+  apply Int.natAbs_lt_natAbs_of_nonneg_of_lt (le_of_lt curpos')
+  exact Int.lt_add_of_pos_right _ incpos'
+
+-- The state and constraints required for the 'mark_multiples' loop
+structure MarkMultiplesState where
+  A : Array Int32
+  inc : Int32
+  cur : Int32
+  incdvd : inc.toInt ∣ cur.toInt
+  curpos : 0 < cur.toInt
+  incpos : 0 < inc.toInt
+  hAslt : A.size < 2^30
+  hmarked : ∀ (j : ℕ),
+    (jpos : 0 < j) → (jlt : j < min cur.toInt A.size) → inc.toInt ∣ (j : ℤ) →
+    A[j]'(Int.lt_of_ofNat_lt_ofNat ((lt_min_iff.mp jlt).2)) ≠ 0
+
+def mark_multiples_state_of_sieve {L : ℕ} (S : Sieve L) : MarkMultiplesState where
+  A := S.divs
+  inc := S.i
+  cur := S.i
+  incdvd := by simp
+  curpos := S.hipos
+  incpos := S.hipos
+  hAslt := by rw [S.hsize]; exact S.hLlt
   hmarked := by
-    intro q qmem i ipos
+    intro j jpos jlt dvdj
+    have jlti := (lt_min_iff.mp jlt).1
+    have lej : 1 ≤ j := Nat.add_one_le_of_lt jpos
+    -- Every entry in the sieve between 1 and i is marked
+    apply sieve_marked_of_lt_index S j (lt_of_le_of_ne lej _) jlti
+    intro j1; subst j1
+    -- Now handle the case where j = 1
+    -- This leads to a contradiction because i ∣ j and 1 < i
+    exact not_lt_of_ge (Int.le_of_dvd (by simp) dvdj) jlti
+
+@[simp] theorem mark_multiples_state_of_sieve_size {L : ℕ} (S : Sieve L) :
+  (mark_multiples_state_of_sieve S).A.size = S.divs.size := rfl
+
+-- When adding 'inc' to 'cur' we can move the addition across the 'toInt' conversion
+lemma mms_cur_add_inc_toInt
+  (MMS : MarkMultiplesState) (curlt : MMS.cur.toInt.natAbs < MMS.A.size) :
+  (MMS.cur + MMS.inc).toInt = MMS.cur.toInt + MMS.inc.toInt := by
+  have curnn : 0 ≤ MMS.cur.toInt := le_of_lt MMS.curpos
+  have incnn : 0 ≤ MMS.inc.toInt := le_of_lt MMS.incpos
+  have curlt' : MMS.cur.toInt < MMS.A.size := by
+    convert Int.ofNat_lt_ofNat_of_lt curlt
+    exact (Int.ofNat_natAbs_of_nonneg curnn).symm
+  have incle := Int.le_of_dvd MMS.curpos MMS.incdvd
+  have inclt' := lt_of_le_of_lt incle curlt'
+  apply int32_toInt_add_of_add_bounds curnn curlt' incnn inclt' (by simp)
+  rw [Int.ofNat_add_ofNat]
+  convert Int.ofNat_le_ofNat_of_le (le_of_lt (Nat.add_lt_add MMS.hAslt MMS.hAslt)) using 1
+
+-- Advance the loop marking multiples of MMS.inc in MMS.A
+def mark_multiples_advance (MMS : MarkMultiplesState)
+  (curlt : MMS.cur.toInt.natAbs < MMS.A.size) : MarkMultiplesState where
+  A := if MMS.A[MMS.cur.toInt.natAbs]'curlt ≠ 0 then MMS.A
+    else MMS.A.set MMS.cur.toInt.natAbs MMS.inc
+  inc := MMS.inc
+  cur := MMS.cur + MMS.inc
+  incdvd := by
+    rw [mms_cur_add_inc_toInt MMS curlt]
+    exact Int.dvd_add MMS.incdvd (by simp)
+  curpos := by
+    rw [mms_cur_add_inc_toInt MMS curlt]
+    exact Int.add_lt_add MMS.curpos MMS.incpos
+  incpos := MMS.incpos
+  hAslt := by
+    convert MMS.hAslt using 1
     split_ifs with h
-    · intro ilt qdvd
-      exact S.hmarked q qmem i ipos ilt qdvd
-    · intro ilt qdvd
-      rw [Array.getElem_set nlt ilt]
-      split_ifs with h'
-      · intro h
-        absurd S.hppos
-        rw [h]; simp
-      · rw [Array.size_set nlt] at ilt
-        exact S.hmarked q qmem i ipos ilt qdvd
-  hpmem_iff := S.hpmem_iff
-  hdivs_dvd := by
-    intro i
+    · rfl
+    · exact Array.size_set curlt
+  hmarked := by
+    -- TODO: This proof seems much longer than necessary.
+    -- Is there anything we can do to shorten / simplify it?
+    intro j jpos jlt jdvd
+    have := mms_cur_add_inc_toInt MMS curlt
+    have incnz : MMS.inc ≠ 0 := by
+      intro hz
+      absurd Int32.toInt_inj.mpr hz; push_neg; symm
+      exact ne_of_lt MMS.incpos
+    by_cases jlt' : j < min MMS.cur.toInt MMS.A.size
+    · obtain ⟨jlt_left, jlt_right⟩ := Int.lt_min.mp jlt'
+      have jlt_left := (Int.lt_min.mp jlt').1
+      have jlt_right := Int.lt_of_ofNat_lt_ofNat (Int.lt_min.mp jlt').2
+      have hAjnz : MMS.A[j]'jlt_right ≠ 0 := by
+        exact MMS.hmarked j jpos jlt' jdvd
+      split_ifs with h
+      · assumption
+      · by_cases curj : MMS.cur.toInt.natAbs = j
+        · rwa [← getElem_congr_idx curj, Array.getElem_set_self]
+          convert curlt using 1
+          exact Array.size_set curlt
+        push_neg at curj
+        rwa [Array.getElem_set_ne curlt jlt_right curj]
+    rename' jlt' => jlb; push_neg at jlb
+    have curlt' := Int.ofNat_lt_ofNat_of_lt curlt
+    rw [Int.ofNat_natAbs_of_nonneg (le_of_lt MMS.curpos)] at curlt'
+    rw [Int.min_eq_left (le_of_lt curlt')] at jlb
+    have jlt' := this ▸ (Int.lt_min.mp jlt).1
+    -- Rewrite 'j' and 'cur' as multiples of 'inc' to prove cur = j
+    rcases dvd_def.mp jdvd with ⟨kj, hkj⟩
+    rcases dvd_def.mp MMS.incdvd with ⟨kcur, hkcur⟩
+    rw [hkj, hkcur] at jlt' jlb
+    rw [Int.mul_le_mul_left MMS.incpos] at jlb
+    nth_rw 3 [← mul_one MMS.inc.toInt] at jlt'
+    rw [← mul_add, Int.mul_lt_mul_left MMS.incpos] at jlt'
+    have hks := le_antisymm (Int.le_of_lt_add_one jlt') jlb
+    rw [hks] at hkj
+    rw [← hkj] at hkcur
+    rename' hkcur => curj
+    have curj' : MMS.cur.toInt.natAbs = j := by
+      rw [curj]; simp
     split_ifs with h
-    · intro ilt hinz
-      exact S.hdivs_dvd i ilt hinz
-    · intro ilt hinz
-      rw [Array.getElem_set nlt ilt] at *
-      split_ifs with h'
-      · subst h'
-        use Int.dvd_natAbs.mpr hdvd
-        intro y lty ydvd
-        /- By contradiction:
-          Suppose y < p. Since 1 < y, there exists a prime 'q' such that q ∣ y
-          but because y ∣ n, q ∣ n. By 'hnextp' we can conclude that q ∈ S.primes
-          Then by 'S.hmarked', because q ∈ S.primes and q ∣ n, S.divs[n] ≠ 0
-          which is a contradiction
-        -/
-        contrapose! h
-        rcases Nat.exists_prime_and_dvd (Nat.ne_of_lt lty).symm with ⟨q, qprime, qdvdy⟩
-        have qdvdn : q ∣ n.toInt.natAbs := Nat.dvd_trans qdvdy ydvd
-        have nabspos : 0 < n.toInt.natAbs := by
-          apply Int.natAbs_pos.mpr
-          apply int32_toInt_ne_zero_of_ne_zero
-          exact (Int32.ne_of_lt hnpos).symm
-        have qley : q ≤ y := Nat.le_of_dvd (lt_trans (by norm_num) lty) qdvdy
-        have qmem := S.hpnext q qprime (lt_of_le_of_lt (Int.ofNat_le_ofNat_of_le qley) h)
-        rcases Array.exists_of_mem_map qmem with ⟨m, mmem, hmq⟩
-        apply S.hmarked m mmem _ nabspos nlt
-        rw [hmq]
-        exact Int.ofNat_dvd.mpr qdvdn
-      · rw [if_neg h'] at hinz
-        rw [Array.size_set nlt] at ilt
-        exact S.hdivs_dvd i ilt hinz
-
-@[simp] theorem mark_sieve_divs_size {L : ℕ} (S : Sieve L) (n : Int32)
-  (hnpos : 0 < n)
-  (nlt : n.toInt.natAbs < S.divs.size)
-  (hdvd : S.p.toInt ∣ n.toInt) :
-  (mark_sieve S n hnpos nlt hdvd).divs.size = S.divs.size := by
-  rw [Sieve.hsize, Sieve.hsize]
-
-@[simp] theorem mark_sieve_primes {L : ℕ} (S : Sieve L) (n : Int32)
-  (hnpos : 0 < n)
-  (nlt : n.toInt.natAbs < S.divs.size)
-  (hdvd : S.p.toInt ∣ n.toInt) :
-  (mark_sieve S n hnpos nlt hdvd).primes = S.primes := rfl
-
-@[simp] theorem mark_sieve_next_prime {L : ℕ} (S : Sieve L) (n : Int32)
-  (hnpos : 0 < n)
-  (nlt : n.toInt.natAbs < S.divs.size)
-  (hdvd : S.p.toInt ∣ n.toInt) :
-  (mark_sieve S n hnpos nlt hdvd).p = S.p := rfl
-
--- Every cell marked in 'S' is also marked in 'mark_sieve S'
-theorem mark_sieve_marked_of_marked {L : ℕ} (S : Sieve L) (n : Int32)
-  (hnpos : 0 < n)
-  (nlt : n.toInt.natAbs < S.divs.size)
-  (hdvd : S.p.toInt ∣ n.toInt) :
-  ∀ i, (ilt : i < S.divs.size) → S.divs[i]'ilt ≠ 0 →
-  (mark_sieve S n hnpos nlt hdvd).divs[i]'(by simpa) ≠ 0 := by
-  intro i ilt hmark
-  unfold mark_sieve; simp
-  split_ifs with h
-  · have hnnein : n.toInt.natAbs ≠ i := by
-      contrapose! hmark
-      subst hmark
+    · rw [← getElem_congr_idx curj']
       assumption
-    rw [Array.getElem_set_ne] <;> assumption
-  · exact hmark
+    · rwa [← getElem_congr_idx curj', Array.getElem_set_self]
+      rwa [Array.size_set]
 
--- The given index is non-zero after calling 'mark_sieve'
-theorem mark_sieve_index_marked {L : ℕ} (S : Sieve L) (n : Int32)
-  (hnpos : 0 < n)
-  (nlt : n.toInt.natAbs < S.divs.size)
-  (hdvd : S.p.toInt ∣ n.toInt) :
-  (mark_sieve S n hnpos nlt hdvd).divs[n.toInt.natAbs]'(by simpa) ≠ 0 := by
-  unfold mark_sieve; dsimp
-  split_ifs with h
-  · rw [Array.getElem_set]; simp
-    intro hpz
-    absurd S.hppos
-    rw [hpz]; simp
-  · assumption
+-- The size of the MarkMultiplesState doesn't change upon advancing
+theorem mark_multiples_advance_size (MMS : MarkMultiplesState)
+  (curlt : MMS.cur.toInt.natAbs < MMS.A.size) :
+  (mark_multiples_advance MMS curlt).A.size = MMS.A.size := by
+  unfold mark_multiples_advance; dsimp
+  split_ifs with h <;> simp
 
-lemma int32_toInt_lt_of_lt_divs_size {L : ℕ} (S : Sieve L) (n : Int32)
-  (hnlt : n.toInt.natAbs < S.divs.size) : n.toInt < 2^30 := by
-  by_cases h : n.toInt ≤ 0
-  · apply lt_of_le_of_lt h (by simp)
-  push_neg at h
-  apply Int.ofNat_lt.mpr at hnlt
-  rw [Int.natAbs_of_nonneg (le_of_lt h), S.hsize] at hnlt
-  exact lt_trans hnlt (Int.ofNat_lt_ofNat_of_lt S.hLlt)
+-- After advancing the MarkMultiplesState, the new 'cur' value is
+-- the sum of the old 'cur' value and the old 'inc' value
+theorem mark_multiples_advance_cur_add_inc (MMS : MarkMultiplesState)
+  (curlt : MMS.cur.toInt.natAbs < MMS.A.size) :
+  (mark_multiples_advance MMS curlt).cur.toInt = MMS.cur.toInt + MMS.inc.toInt := by
+  unfold mark_multiples_advance; dsimp
+  exact mms_cur_add_inc_toInt MMS curlt
 
--- We'll need this result below for "mark_multiples"
-lemma int32_toInt_add_of_pos_of_dvd_of_lt (m n : Int32)
-  (hmpos : 0 < m) (hnpos : 0 < n)
-  (hdvd : m.toInt ∣ n.toInt) (hnlt : n.toInt < 2^30) :
-  (m + n).toInt = m.toInt + n.toInt := by
-  have hmpos' := int32_toInt_pos_of_pos hmpos
-  have hnpos' := int32_toInt_pos_of_pos hnpos
-  apply int32_toInt_add_of_bounds
-  constructor
-  · apply le_of_lt
-    exact lt_trans (by simp) (Int.add_lt_add hmpos' hnpos')
-  · rw [add_comm]
-    apply lt_of_le_of_lt (Int.add_le_add_left (Int.le_of_dvd hnpos' hdvd) n.toInt)
-    rw [← two_mul, Int.pow_succ, mul_comm]
-    exact (Int.mul_lt_mul_right (two_pos)).mpr hnlt
+-- Prove 'mark_multiples' terminates
+lemma mark_multiples_terminates (MMS : MarkMultiplesState)
+  (curlt : MMS.cur.toInt.natAbs < MMS.A.size) :
+  (fun f mms' ↦ f mms' < f MMS)
+  (fun mms ↦ mms.A.size - mms.cur.toInt.natAbs)
+  (mark_multiples_advance MMS curlt) := by
+  dsimp
+  rw [mark_multiples_advance_size, mark_multiples_advance_cur_add_inc]
+  apply Nat.sub_lt_sub_left curlt
+  apply Int.natAbs_lt_natAbs_of_nonneg_of_lt (le_of_lt MMS.curpos)
+  exact Int.lt_add_of_pos_right _ MMS.incpos
 
--- Useful alternate upper bound on 'n'
-lemma sieve_idx_lt_divs_size
-  {L : ℕ} (S : Sieve L) (n : Int32)
-  (hnnn : 0 ≤ n) (hnlt : n.toInt < (L : ℤ)) :
-  n.toInt.natAbs < S.divs.size := by
-  apply Int.lt_of_ofNat_lt_ofNat
-  rw [S.hsize]
-  convert hnlt
-  have hnnn' := Int32.le_iff_toInt_le.mp hnnn
-  exact Int.ofNat_natAbs_of_nonneg hnnn'
-
--- General strategy for proving termination when iterating over the sieve
-lemma sieve_termination {L : ℕ} (S : Sieve L) (n m : Int32)
-  (hnpos : 0 < n) (hmpos : 0 < m)
-  (hnlt : n.toInt.natAbs < S.divs.size) (hmle : m ≤ n) :
-  S.divs.size - (n + m).toInt.natAbs < S.divs.size - n.toInt.natAbs := by
-  have hnpos' : 0 < n.toInt := int32_toInt_pos_of_pos hnpos
-  have hmpos' : 0 < m.toInt := int32_toInt_pos_of_pos hmpos
-  have hnub : n.toInt < 2 ^ 30 := int32_toInt_lt_of_lt_divs_size S n hnlt
-  have hmub : m.toInt < 2 ^ 30 :=
-    lt_of_le_of_lt (Int32.le_iff_toInt_le.mp hmle) hnub
-  have hnm : (n + m).toInt = n.toInt + m.toInt := by
-    rw [int32_toInt_add_of_bounds]
-    constructor
-    · exact le_trans (by simp) (le_of_lt (Int.add_lt_add hnpos' hmpos'))
-    · exact Int.add_lt_add hnub hmub
-  rw [hnm]
-  apply Nat.sub_lt_sub_left hnlt
-  apply Int.natAbs_lt_natAbs_of_nonneg_of_lt (le_of_lt hnpos')
-  exact Int.lt_add_of_pos_right _ hmpos'
-
--- Prove the termination requirements for 'mark_multiple'
-lemma mark_multiple_termination {L : ℕ} (S : Sieve L) (n : Int32)
-  (hnpos : 0 < n)
-  (hdvd : S.p.toInt ∣ n.toInt)
-  (hnlt : n.toInt.natAbs < S.divs.size) :
-  S.divs.size - (n + S.p).toInt.natAbs < S.divs.size - n.toInt.natAbs := by
-  have hnpos' := int32_toInt_pos_of_pos hnpos
-  apply sieve_termination S _ _ hnpos S.hppos hnlt
-  exact Int32.le_iff_toInt_le.mpr (Int.le_of_dvd hnpos' hdvd)
-
--- Mark one multiple of 'p' in sieve 'S'
-def mark_multiple {L : ℕ} (S : Sieve L) (n : Int32)
-  (hnpos : 0 < n)
-  (hdvd : S.p.toInt ∣ n.toInt) : Sieve L :=
-  if hnlt : n.toInt.natAbs < S.divs.size then
-  (fun (hnp : (n + S.p).toInt = n.toInt + S.p.toInt) ↦
-    mark_multiple
-      (mark_sieve S n hnpos hnlt hdvd)
-      (n + S.p) (by
-        apply Int32.lt_iff_toInt_lt.mpr
-        rw [hnp]
-        apply Int.add_pos (Int32.lt_iff_toInt_lt.mp hnpos)
-        exact Int32.lt_iff_toInt_lt.mp S.hppos
-      ) (by
-        rw [hnp]
-        exact Int.dvd_add hdvd (by use 1; simp)
-      ))
-  (by
-    have hppos' := int32_toInt_pos_of_pos S.hppos
-    have hnpos' := int32_toInt_pos_of_pos hnpos
-    rw [Int.add_comm, Int32.add_comm]
-    apply int32_toInt_add_of_pos_of_dvd_of_lt S.p n S.hppos hnpos hdvd
-    exact int32_toInt_lt_of_lt_divs_size S _ hnlt
-  ) else S
-termination_by S.divs.size - n.toInt.natAbs
+def mark_multiples_impl (MMS : MarkMultiplesState) : MarkMultiplesState :=
+  if curlt : MMS.cur.toInt.natAbs < MMS.A.size then
+    mark_multiples_impl (mark_multiples_advance MMS curlt) else
+    MMS
+termination_by MMS.A.size - MMS.cur.toInt.natAbs
 decreasing_by
-  rw [mark_sieve_divs_size]
-  apply mark_multiple_termination <;> assumption
+  exact mark_multiples_terminates MMS curlt
 
--- Mark all multiples of the next prime, 'p', in the Sieve
-def mark_multiples {L : ℕ} (S : Sieve L) : Sieve L :=
-  mark_multiple S S.p S.hppos (by use 1; simp)
-
-@[simp] theorem mark_multiple_divs_size {L : ℕ} (S : Sieve L) (n : Int32)
-  (hnpos : 0 < n)
-  (hdvd : S.p.toInt ∣ n.toInt) :
-  (mark_multiple S n hnpos hdvd).divs.size = S.divs.size := by
-  rw [Sieve.hsize, Sieve.hsize]
-
--- The 'primes' field is unchanged by 'mark_multiple'
-@[simp] theorem mark_multiple_primes {L : ℕ} (S : Sieve L) (n : Int32)
-  (hnpos : 0 < n)
-  (hdvd : S.p.toInt ∣ n.toInt) :
-  (mark_multiple S n hnpos hdvd).primes = S.primes := by
-  unfold mark_multiple; simp
+theorem mark_multiples_impl_size (MMS : MarkMultiplesState) :
+  (mark_multiples_impl MMS).A.size = MMS.A.size := by
+  unfold mark_multiples_impl
   split_ifs with h
-  · apply mark_multiple_primes
+  · rw [mark_multiples_impl_size, mark_multiples_advance_size]
   · rfl
-termination_by S.divs.size - n.toInt.natAbs
+termination_by MMS.A.size - MMS.cur.toInt.natAbs
 decreasing_by
-  rw [mark_sieve_divs_size]
-  apply mark_multiple_termination <;> assumption
+  exact mark_multiples_terminates MMS h
 
--- Every cell marked in 'S' is also marked in 'mark_multiple S'
-theorem mark_multiple_marked_of_marked {L : ℕ} (S : Sieve L) (n : Int32)
-  (hnpos : 0 < n)
-  (hdvd : S.p.toInt ∣ n.toInt) :
-  ∀ i, (ilt : i < S.divs.size) → S.divs[i]'ilt ≠ 0 →
-  (mark_multiple S n hnpos hdvd).divs[i]'(by simpa) ≠ 0 := by
-  intro i ilt hmark
-  unfold mark_multiple; dsimp
-  split_ifs with h
-  · push_neg
-    apply mark_multiple_marked_of_marked
-    · apply mark_sieve_marked_of_marked <;> assumption
-  · exact hmark
-termination_by S.divs.size - n.toInt.natAbs
-decreasing_by
-  rw [mark_sieve_divs_size]
-  apply mark_multiple_termination <;> assumption
+-- Extract S.divs and mark every entry which is a multiple of S.i
+def mark_multiples {L : ℕ} (S : Sieve L) : MarkMultiplesState :=
+  mark_multiples_impl (mark_multiples_state_of_sieve S)
 
--- Show that 'mark_multiple' does indeed mark every
--- multiple of 'p' greater than or equal to 'n'
-theorem mark_multiple_verify {L : ℕ} (S : Sieve L) (n : Int32)
-  (hnpos : 0 < n)
-  (hdvd : S.p.toInt ∣ n.toInt) :
-  ∀ (i : ℕ), (n.toInt ≤ (i : ℤ)) → (ilt : i < S.divs.size) →
-    S.p.toInt ∣ (i : ℤ) →
-  (mark_multiple S n hnpos hdvd).divs[i]'(by
-    rwa [mark_multiple_divs_size]
-  ) ≠ 0 := by
-  have hppos' := int32_toInt_pos_of_pos S.hppos
-  have hnpos' := int32_toInt_pos_of_pos hnpos
-  have hnabs : (n.toInt.natAbs : ℤ) = n.toInt := Int.natAbs_of_nonneg (le_of_lt hnpos')
-  intro i nlei ilt pdvdi
-  unfold mark_multiple
-  split_ifs with h
-  · simp; push_neg
-    have hnlt : n.toInt < 2^30 :=
-      int32_toInt_lt_of_lt_divs_size S _ h
-    have ipos : 0 < (i : ℤ) :=
-      lt_of_lt_of_le (int32_toInt_pos_of_pos hnpos) nlei
-    have := int32_toInt_add_of_pos_of_dvd_of_lt S.p n S.hppos hnpos hdvd hnlt
-    rw [Int.add_comm, Int32.add_comm] at this
-    have hnppos : 0 < n + S.p := by
-      apply Int32.lt_iff_toInt_lt.mpr
-      rw [this]; simp
-      exact Int.add_pos hnpos' hppos'
-    have hdvd' : S.p.toInt ∣ (n + S.p).toInt := by
-      rw [this]
-      exact Int.dvd_add hdvd (by use 1; simp)
-    let S' := (mark_sieve S n hnpos h hdvd)
-    have hnextp' :
-      ∀ (q : ℕ), Nat.Prime q → ↑q < S.p.toInt → ↑q ∈ Array.map Int32.toInt S'.primes := by
-      intro q qprime qlt
-      unfold S'
-      rw [mark_sieve_primes]
-      exact S.hpnext q qprime qlt
-    by_cases hnple : (n + S.p).toInt ≤ (i : ℤ)
-    · apply mark_multiple_verify S' (n + S.p) hnppos hdvd' i hnple _ pdvdi
-      unfold S'; simpa
-    rename' hnple => ilt'; push_neg at ilt'
-    -- At this point, from nlei, ilt', and pdvdi we can conclude that i = n
-    rw [this] at ilt'
-    rcases pdvdi with ⟨ki, hipk⟩
-    have hdvdcp := hdvd
-    rcases hdvdcp with ⟨kn, hnpk⟩
-    rw [hipk, hnpk] at ilt'
-    rw [hipk, hnpk] at nlei
-    nth_rw 3 [← Int.mul_one S.p.toInt] at ilt'
-    rw [← Int.mul_add] at ilt'
-    apply (Int.mul_lt_mul_left hppos').mp at ilt'
-    apply (Int.mul_le_mul_left hppos').mp at nlei
-    have hknki : kn = ki := Int.le_antisymm nlei (Int.le_of_lt_add_one ilt')
-    rw [← hknki, ← hnpk] at hipk
-    rename' hipk => hin
-    apply mark_multiple_marked_of_marked
-    · convert mark_sieve_index_marked S n hnpos h hdvd
-      apply Int.ofNat_inj.mp; symm
-      exact hin ▸ hnabs
-    simpa
-  · intro h'
-    apply h
-    apply lt_of_le_of_lt _ ilt
-    apply Int.le_of_ofNat_le_ofNat
-    rwa [hnabs]
-termination_by S.divs.size - n.toInt.natAbs
-decreasing_by
-  rw [mark_sieve_divs_size]
-  apply mark_multiple_termination <;> assumption
-
--- Verify that 'mark_multiples' does indeed mark every multiple of 'p'
-theorem mark_multiples_verify {L : ℕ} (S : Sieve L) :
-  ∀ (i : ℕ), (0 < i) → (ilt : i < S.divs.size) →
-    S.p.toInt ∣ (i : ℤ) →
-  (mark_multiples S).divs[i]'(by
-    unfold mark_multiples; simpa
-  ) ≠ 0 := by
-  intro i hipos ilt pdvdi
+theorem mark_multiples_size {L : ℕ} (S : Sieve L) :
+  (mark_multiples S).A.size = S.divs.size := by
   unfold mark_multiples
-  have hipos' : 0 < (i : ℤ) := Int.ofNat_lt_ofNat_of_lt hipos
-  have plei := Int.le_of_dvd hipos' pdvdi
-  apply mark_multiple_verify <;> assumption
-
--- Used in 'find_next_prime' below
-lemma int32_toInt_succ_of_lt_sieve_length {L : ℕ} (S : Sieve L)
-  (n : Int32) (hlt : n.toInt < (L : ℤ)) :
-  (n + 1).toInt = n.toInt + 1 := by
-  apply int32_toInt_succ _ (Int32.lt_iff_toInt_lt.mpr _)
-  apply lt_trans hlt (lt_trans (Int.ofNat_lt_ofNat_of_lt S.hLlt) _)
-  unfold Int32.maxValue; simp
-
--- Used in 'find_next_prime' below
-lemma int32_lt_succ_of_lt_sieve_length {L : ℕ} (S : Sieve L)
-  (n : Int32) (hlt : n.toInt < (L : ℤ)) :
-  n < n + 1 := by
-  apply Int32.lt_iff_toInt_lt.mpr
-  convert Int.lt_succ n.toInt
-  exact int32_toInt_succ_of_lt_sieve_length S n hlt
-
--- Prove that 'find_next_prime_impl' (defined below) terminates
--- This will also be used to prove termination for many related proofs
-lemma find_next_prime_impl_termination
-  {L : ℕ} (S : Sieve L) (n : Int32) (hltn : 1 < n) (nlt : n.toInt < (L : ℤ)) :
-  S.divs.size - (n + 1).toInt.natAbs < S.divs.size - n.toInt.natAbs := by
-  have hnpos : 0 < n := Int32.lt_trans (by simp) hltn
-  have nlt' := sieve_idx_lt_divs_size S n (Int32.le_of_lt hnpos) nlt
-  exact sieve_termination S _ _ hnpos (by simp) nlt' (Int32.le_of_lt hltn)
-
--- Loop over the entries in the sieve to find the next prime
-def find_next_prime_impl {L : ℕ} (S : Sieve L)
-  (n : Int32) (hltn : 1 < n) : Int32 :=
-  if nlt : n.toInt < (L : ℤ) then
-  if h : S.divs[n.toInt.natAbs]'(by
-      apply Int.lt_of_ofNat_lt_ofNat
-      convert S.hsize ▸ nlt
-      apply Int.natAbs_of_nonneg (le_of_lt _)
-      apply lt_trans _ (Int32.lt_iff_toInt_lt.mp hltn); simp
-  ) = 0 then n else
-  find_next_prime_impl S (n + 1) (by
-    apply Int32.lt_trans hltn
-    exact int32_lt_succ_of_lt_sieve_length S _ nlt
-  ) else Int32.ofInt (L : ℤ)
-termination_by S.divs.size - n.toInt.natAbs
-decreasing_by
-  apply find_next_prime_impl_termination <;> assumption
-
--- Starting with the current prime, search for the next prime
-def find_next_prime {L : ℕ} (S : Sieve L) : Int32 :=
-  find_next_prime_impl S (S.p + 1) (by
-    apply Int32.lt_iff_toInt_lt.mpr
-    rw [int32_toInt_succ_of_lt_sieve_length S _ S.hplt]; simp
-    exact Int32.lt_iff_toInt_lt.mp S.hppos
-  )
-
--- Prove a lower bound for 'find_next_prime_impl' in the
--- case where the search doesn't reach the end of the sieve
-theorem find_next_prime_impl_lb {L : ℕ} (S : Sieve L)
-  (n : Int32) (hltn : 1 < n) :
-  (fun p ↦ p.toInt ≠ (L : ℤ) → 2 ≤ p.toInt) (find_next_prime_impl S n hltn) := by
-  dsimp; intro pneL
-  unfold find_next_prime_impl at *; dsimp at *
-  split_ifs at * with h₀ h₁
-  · exact Int32.lt_iff_toInt_lt.mp hltn
-  · apply find_next_prime_impl_lb
-    assumption
-  · absurd pneL
-    have Lnn := Int.natCast_nonneg L
-    have ltL : -2^31 ≤ (L : ℤ) := le_trans (by simp) Lnn
-    have Llt : (L : ℤ) < 2^31 :=
-      lt_trans (Int.ofNat_lt_ofNat_of_lt S.hLlt) (by simp)
-    rw [Int32.toInt_ofInt_of_le ltL Llt]
-termination_by S.divs.size - n.toInt.natAbs
-decreasing_by
-  apply find_next_prime_impl_termination <;> assumption
-
--- Prove a lower bound for 'find_next_prime' in the
--- case where the search doesn't reach the end of the sieve
-theorem find_next_prime_lb {L : ℕ} (S : Sieve L) :
-  (fun p ↦ p.toInt ≠ (L : ℤ) → 2 ≤ p.toInt) (find_next_prime S) := by
-  dsimp; intro pneL
-  unfold find_next_prime at *
-  apply find_next_prime_impl_lb
-  assumption
-
--- 'find_next_prime_impl' always returns a non-negative integer
-theorem find_next_prime_impl_nonneg {L : ℕ} (S : Sieve L)
-  (n : Int32) (hltn : 1 < n) :
-  0 ≤ (find_next_prime_impl S n hltn).toInt := by
-  unfold find_next_prime_impl; dsimp
-  split_ifs with h₀ h₁
-  · exact le_of_lt (lt_trans (by simp) (Int32.lt_iff_toInt_lt.mp hltn))
-  · apply find_next_prime_impl_nonneg
-  · have Lnn := Int.natCast_nonneg L
-    have ltL : -2^31 ≤ (L : ℤ) := le_trans (by simp) Lnn
-    rwa [Int32.toInt_ofInt_of_le ltL]
-    exact lt_trans (Int.ofNat_lt_ofNat_of_lt S.hLlt) (by simp)
-termination_by S.divs.size - n.toInt.natAbs
-decreasing_by
-  apply find_next_prime_impl_termination <;> assumption
-
--- 'find_next_prime' always returns a non-negative integer
-theorem find_next_prime_nonneg {L : ℕ} (S : Sieve L) :
-  0 ≤ (find_next_prime S).toInt := by
-  unfold find_next_prime
-  apply find_next_prime_impl_nonneg
-
--- For the length of the sieve, Int32.ofInt and Int32.toInt are inverses
-lemma sieve_length_toInt_ofInt {L : ℕ} (S : Sieve L) :
-  (Int32.ofInt (L : ℤ)).toInt = (L : ℤ) := by
-  apply Int32.toInt_ofInt_of_le
-  · exact le_trans (by simp) (Int.natCast_nonneg L)
-  · exact lt_trans (Int.ofNat_lt_ofNat_of_lt S.hLlt) (by simp)
-
--- 'find_next_prime_impl' finds an unmarked entry in the sieve
--- if its search doesn't reach the end of the sieve
-theorem find_next_prime_impl_unmarked {L : ℕ} (S : Sieve L)
-  (n : Int32) (hltn : 1 < n) :
-  (fun p (pnn : 0 ≤ p) ↦ (h : p.toInt < (L : ℤ)) →
-    S.divs[p.toInt.natAbs]'(sieve_idx_lt_divs_size S p pnn h) = 0
-  ) (find_next_prime_impl S n hltn) (by
-    apply Int32.le_iff_toInt_le.mpr
-    exact find_next_prime_impl_nonneg S n hltn
-  ) := by
-  dsimp
-  intro h
-  unfold find_next_prime_impl; dsimp
-  split_ifs with h₀ h₁
-  · exact h₁
-  · unfold find_next_prime_impl at h; dsimp at h
-    rw [dif_pos h₀, if_neg h₁] at h
-    apply find_next_prime_impl_unmarked
-    assumption
-  · unfold find_next_prime_impl at h; dsimp at h
-    rw [dif_neg h₀] at h
-    absurd h; push_neg
-    apply Int.le_of_eq; symm
-    exact sieve_length_toInt_ofInt S
-termination_by S.divs.size - n.toInt.natAbs
-decreasing_by
-  apply find_next_prime_impl_termination <;> assumption
-
--- 'find_next_prime' finds an unmarked entry in the sieve
--- if its search doesn't reach the end of the sieve
-theorem find_next_prime_unmarked {L : ℕ} (S : Sieve L) :
-  (fun p (pnn : 0 ≤ p) ↦ (h : p.toInt < (L : ℤ)) →
-    S.divs[p.toInt.natAbs]'(
-      sieve_idx_lt_divs_size S p pnn h
-    ) = 0
-  ) (find_next_prime S) (by
-    apply Int32.le_iff_toInt_le.mpr
-    exact find_next_prime_nonneg S
-  ) := by
-  dsimp
-  intro h
-  unfold find_next_prime at *
-  apply find_next_prime_impl_unmarked
-  assumption
-
--- The value of 'find_next_prime_impl' does not exceed 'L'
-theorem find_next_prime_impl_ub
-  {L : ℕ} (S : Sieve L) (n : Int32) (hltn : 1 < n) :
-  (find_next_prime_impl S n hltn).toInt ≤ (L : ℤ) := by
-  unfold find_next_prime_impl; dsimp
-  split_ifs with h₀ h₁
-  · exact le_of_lt h₀
-  · apply find_next_prime_impl_ub
-  · apply Int.le_of_eq
-    exact sieve_length_toInt_ofInt S
-termination_by S.divs.size - n.toInt.natAbs
-decreasing_by
-  apply find_next_prime_impl_termination <;> assumption
-
--- The value of 'find_next_prime' does not exceed 'L'
-theorem find_next_prime_ub {L : ℕ} (S : Sieve L) :
-  (find_next_prime S).toInt ≤ (L : ℤ) := by
-  unfold find_next_prime
-  apply find_next_prime_impl_ub
-
--- Every entry between the starting point of the search and
--- the value returned by 'find_next_prime_impl' is marked
-theorem find_next_prime_impl_first_unmarked
-  {L : ℕ} (S : Sieve L) (n : Int32) (hltn : 1 < n) :
-  ∀ (i : ℕ), n.toInt ≤ (i : ℤ) →
-  (ilt : (i : ℤ) < (find_next_prime_impl S n hltn).toInt) →
-  S.divs[i]'(by
-    rw [S.hsize]
-    apply Int.lt_of_ofNat_lt_ofNat (lt_of_lt_of_le ilt _)
-    apply find_next_prime_impl_ub
-  ) ≠ 0 := by
-  intro i nlei ilt
-  have ilt' : i < L := by
-    apply Int.lt_of_ofNat_lt_ofNat
-    apply lt_of_lt_of_le ilt
-    apply find_next_prime_impl_ub
-  unfold find_next_prime_impl at ilt; dsimp at ilt
-  split_ifs at ilt with h₀ h₁
-  · absurd nlei; push_neg
-    assumption
-  · by_cases hni : n.toInt = (i : ℤ)
-    · convert h₁
-      rw [hni]; simp
-    have hnlti : n.toInt < (i : ℤ) := lt_of_le_of_ne nlei hni
-    have hltns : 1 < n + 1 := by
-      apply Int32.lt_trans hltn
-      exact int32_lt_succ_of_lt_sieve_length S n h₀
-    apply find_next_prime_impl_first_unmarked S (n + 1) hltns i _ ilt
-    rw [int32_toInt_succ_of_lt_sieve_length S n h₀]
-    exact Int.add_one_le_of_lt hnlti
-  · absurd nlei; push_neg
-    apply lt_of_lt_of_le _ (le_of_not_gt h₀)
-    exact Int.ofNat_lt_ofNat_of_lt ilt'
-termination_by S.divs.size - n.toInt.natAbs
-decreasing_by
-  apply find_next_prime_impl_termination <;> assumption
-
--- Every entry between the starting point of the search and
--- the value returned by 'find_next_prime_impl' is marked
-theorem find_next_prime_first_unmarked
-  {L : ℕ} (S : Sieve L) :
-  ∀ (i : ℕ), S.p.toInt + 1 ≤ (i : ℤ) →
-  (ilt : (i : ℤ) < (find_next_prime S).toInt) →
-  S.divs[i]'(by
-    rw [S.hsize]
-    apply Int.lt_of_ofNat_lt_ofNat (lt_of_lt_of_le ilt _)
-    apply find_next_prime_ub
-  ) ≠ 0 := by
-  intro i plti ilt
-  unfold find_next_prime at ilt
-  rw [← int32_toInt_succ_of_lt_sieve_length S S.p S.hplt] at plti
-  apply find_next_prime_impl_first_unmarked S (S.p + 1) _ i plti ilt
+  rw [mark_multiples_impl_size]; simp
 
 end CodeChef
